----------------------------------------------------------------------
Committing in a revised version of the quotients package, and an example.

The quotient theorems are broken into theories based on the type operator
they refer to, with general non-specific theorems remaining in
quotientScript.sml.

The example of creating finite sets from lists by a quotient is presented
in the new "examples" directory, in finite_setScript.sml.  It is perhaps
surprisingly simple to walk through.

Modified Files:
	hol98/src/quotient/src/quotient.sml
	hol98/src/quotient/src/quotientLib.sml
	hol98/src/quotient/src/quotientScript.sml
	hol98/src/quotient/src/quotient_listScript.sml
	hol98/src/quotient/src/quotient_optionScript.sml
	hol98/src/quotient/src/quotient_pairScript.sml
	hol98/src/quotient/src/quotient_sumScript.sml
Added Files:
	hol98/src/quotient/examples/finite_setScript.sml
	hol98/src/quotient/examples/ind_rel.sig
	hol98/src/quotient/examples/ind_rel.sml
	hol98/src/quotient/src/quotient_pred_setScript.sml
----------------------------------------------------------------------

src/quotient/examples/ind_rel.sig
@@ -1,0 +1,28 @@
+(* Subject: Mutually recursive rule induction *)
+(* Author: Myra Van Inwegen *)
+(* Part of the author's doctoral dissertation *)
+
+signature ind_rel =
+sig
+
+val   check_inductive_relations :
+         Term.term list ->     (* patterns *)
+         Term.term ->          (* term giving rules *)
+         Term.term list        (* each term corresponds to a quantified rule *)
+val   define_inductive_relations :
+         Term.term list ->     (* patterns *)
+         Term.term ->          (* term giving rules *)
+         Thm.thm * Thm.thm     (* rules_satisfied theorem, induction theorem *)
+val   prove_inversion_theorems : 
+         Thm.thm ->            (* rules_satisfied theorem *)
+         Thm.thm ->            (* induction theorem *)
+         Thm.thm list          (* inversion theorems *)
+val   prove_strong_induction :
+         Thm.thm ->            (* rules_satisfied theorem *)
+         Thm.thm ->            (* induction theorem *)
+         Thm.thm               (* strong induction theorem *)
+val   rule_induct :
+         Thm.thm ->            (* induction theorem (strong or regular) *)
+	 Abbrev.tactic         (* sets up induction *)
+
+end;
