src/quotient/src/quotientLib.sml
@@ -5,6 +5,7 @@ struct
    open quotient_pairTheory
    open quotient_sumTheory
    open quotient_optionTheory
+   open quotient_pred_setTheory
    open quotient
 end
 
