src/quotient/src/quotientScript.sml
@@ -4,9 +4,9 @@ infixr -->;
 
 
 (* --------------------------------------------------------------------- *)
-(* Lifting the lambda calculus syntax to the abstract level.             *)
-(* Version 2.1.                                                          *)
-(* Date: February 28, 2005                                               *)
+(* Fundamental definitions and theorems for the quotients package.       *)
+(* Version 2.2.                                                          *)
+(* Date: April 11, 2005                                                  *)
 (* --------------------------------------------------------------------- *)
 
 
@@ -47,6 +47,15 @@ val POP_TAC = POP_ASSUM (fn th => ALL_TAC);
 (* =================================================================== *)
 
 
+
+(* Equivalence relations: *)
+
+val EQUIV_def =
+    Define
+      `EQUIV E = !x y:'a. E x y = (E x = E y)`;
+
+(* Quotients, with partial equivalence relation, abstraction function, and
+   representation function: *)
 
 val QUOTIENT_def =
     Define
@@ -126,8 +135,9 @@ val QUOTIENT_REP_ABS = store_thm
 
 val IDENTITY_EQUIV = store_thm
    ("IDENTITY_EQUIV",
-    (--`!x y:'a. (x = y) = ($= x = $= y)`--),
-    REPEAT GEN_TAC
+    (--`EQUIV ($= : 'a -> 'a -> bool)`--),
+    REWRITE_TAC[EQUIV_def]
+    THEN REPEAT GEN_TAC
     THEN EQ_TAC
     THEN DISCH_THEN REWRITE_THM
    );
@@ -628,152 +638,6 @@ val FUN_REL_IMP = store_thm
     REPEAT STRIP_TAC
     THEN IMP_RES_TAC FUN_REL_EQUALS
    );
-
-
-(* ============================ *)
-(* Main development of SET_REL: *)
-(* ============================ *)
-
-(* for set rep or abs, DON'T use (abs --> I) or (rep --> I).  *)
-(* No, for set rep or abs, use SET_MAP abs or SET_MAP rep.  *)
-
-val SET_REL_def =
-    Define
-      `SET_REL (R:'a->'a->bool) = (R ===> ($= :bool->bool->bool))`;
-
-(*
-val SET_REL_def =
-    Define
-      `SET_REL (R:'a->'a->bool) s t = (R ===> ($= :bool->bool->bool)) s t /\
-                                      (!x. x IN s \/ x IN t ==> respects R x)`;
-*)
-
-val SET_REL = store_thm
-   ("SET_REL",
-    (--`!(R:'a->'a->bool).
-         SET_REL R s t =
-           (!x y. R x y ==> ((x IN s) = (y IN t)))`--),
-    REPEAT GEN_TAC
-    THEN REWRITE_TAC[SET_REL_def,FUN_REL,SPECIFICATION]
-   );
-
-val SET_MAP_def =
-    Define
-      `SET_MAP (f:'a->'b) = (f --> (I:bool->bool))`;
-
-val SET_MAP_COMPOSE = store_thm
-   ("SET_MAP_COMPOSE",
-    (--`!(f:'a->'b) s.
-         SET_MAP f s = s o f`--),
-    REPEAT GEN_TAC
-    THEN REWRITE_TAC[SET_MAP_def,FUN_MAP_THM,I_THM,o_THM,
-                     EXTENSION,SPECIFICATION]
-   );
-
-val IN_SET_MAP = store_thm
-   ("IN_SET_MAP",
-    (--`!(f:'a->'b) s x.
-         x IN SET_MAP f s = f x IN s`--),
-    REPEAT GEN_TAC
-    THEN REWRITE_TAC[SET_MAP_COMPOSE,SPECIFICATION,o_THM]
-   );
-
-val SET_MAP_SET_MAP = store_thm
-   ("SET_MAP_SET_MAP",
-    (--`!(f:'a->'b) (g:'b->'c) s.
-         SET_MAP f (SET_MAP g s) = SET_MAP (g o f) s`--),
-    REPEAT GEN_TAC
-    THEN REWRITE_TAC[SET_MAP_COMPOSE,o_ASSOC]
-   );
-
-val SET_QUOTIENT = store_thm
-   ("SET_QUOTIENT",
-    (--`!R (abs:'a->'c) rep. QUOTIENT R abs rep ==>
-         QUOTIENT (SET_REL R) (SET_MAP rep) (SET_MAP abs)`--),
-    REPEAT GEN_TAC
-    THEN STRIP_TAC
-    THEN REWRITE_TAC[SET_REL_def,SET_MAP_def]
-    THEN IMP_RES_THEN MATCH_MP_TAC FUN_QUOTIENT
-    THEN REWRITE_TAC[IDENTITY_QUOTIENT]
-   );
-
-
-val SET_REL_MP = store_thm
-   ("SET_REL_MP",
-    (--`!(R:'a -> 'a -> bool) s t x y.
-         (SET_REL R) s t ==> R x y ==> (x IN s = y IN t)`--),
-    REPEAT STRIP_TAC
-    THEN IMP_RES_TAC SET_REL
-   );
-
-
-(* One possible development of SET_REL, based on set rep/abs by IMAGE:
-Unfortunately this definition makes it impossible to prove the respectfulness
-theorems for such operators as IN.
-
-val SET_REL_def =
-    Define
-      `SET_REL (R:'a->'a->bool) s t =
-                     (!x. x IN s ==> ?y. y IN t /\ R x y) /\
-                     (!y. y IN t ==> ?x. x IN s /\ R x y)`;
-
-
-val SET_EQUIV = store_thm
-   ("SET_EQUIV",
-    (--`!R :'a->'a->bool.
-         (!x y. R x y = (R x = R y)) ==>
-         (!x y. SET_REL R x y = (SET_REL R x = SET_REL R y))`--),
-    GEN_TAC
-    THEN REWRITE_TAC[EQUIV_REFL_SYM_TRANS]
-    THEN STRIP_TAC
-    THEN REWRITE_TAC[SET_REL_def,EXTENSION,IN_IMAGE]
-    THEN REPEAT STRIP_TAC (* 6 subgoals *)
-    THENL
-      [ EXISTS_TAC ``x':'a``
-        THEN ASM_REWRITE_TAC[],
-
-        EXISTS_TAC ``y:'a``
-        THEN ASM_REWRITE_TAC[],
-
-        RES_TAC
-        THEN EXISTS_TAC ``x'':'a``
-        THEN RES_TAC
-        THEN ASM_REWRITE_TAC[],
-
-        RES_TAC
-        THEN EXISTS_TAC ``y'':'a``
-        THEN RES_TAC
-        THEN ASM_REWRITE_TAC[],
-
-        RES_TAC
-        THEN RES_TAC
-        THEN EXISTS_TAC ``y'':'a``
-        THEN ASM_REWRITE_TAC[],
-
-        RES_TAC
-        THEN RES_TAC
-        THEN EXISTS_TAC ``x''':'a``
-        THEN ASM_REWRITE_TAC[]
-      ]
-    THEN PROVE_TAC[] (* could replace the THENL 6 cases above *)
-   );
-
-
-val SET_QUOTIENT = store_thm
-   ("SET_QUOTIENT",
-    (--`!R (abs:'a->'b) rep.
-         (!a. abs (rep a) = a) /\
-         (!r r'. R r r' = (abs r = abs r')) ==>
-         (!a. IMAGE abs (IMAGE rep a) = a) /\
-         (!r r'. SET_REL R r r' = (IMAGE abs r = IMAGE abs r'))`--),
-    REPEAT GEN_TAC
-    THEN STRIP_TAC
-    THEN CONJ_TAC
-    THEN REWRITE_TAC[SET_REL_def,EXTENSION,IN_IMAGE]
-    THEN PROVE_TAC[]
-   );
-
-*)
 
 
 
@@ -1489,651 +1353,6 @@ val W_RSP = store_thm
 
 
 
-(* pred_set theory: IN, EMPTY, UNIV, INTER, UNION, SUBSET, PSUBSET, IMAGE *)
-
-val IN_PRS = store_thm
-   ("IN_PRS",
-    (--`!R (abs:'a -> 'b) rep. QUOTIENT R abs rep ==>
-         !x s. x IN s =
-               rep x IN SET_MAP abs s`--),
-    REPEAT STRIP_TAC
-    THEN IMP_RES_TAC QUOTIENT_ABS_REP
-    THEN ASM_REWRITE_TAC[IN_SET_MAP]
-   );
-
-val IN_RSP = store_thm
-   ("IN_RSP",
-    (--`!R (abs:'a -> 'b) rep. QUOTIENT R abs rep ==>
-         !x1 x2 s1 s2.
-          R x1 x2 /\ (SET_REL R) s1 s2 ==>
-          (x1 IN s1 = x2 IN s2)`--),
-    REPEAT STRIP_TAC
-    THEN IMP_RES_TAC SET_REL_MP
-   );
-
-
-(* GSPEC does not lift directly; because its definition
-
-GSPECIFICATION   |- !f v. v IN GSPEC f = ?x. (v,T) = f x : thm
-
-involves = between v:'b and FST(f x):'b, rather than R2 v (FST(f x)),
-it does not respect the equivalence relation on 'b.
-But a similar operator exists which we can try to lift to GSPEC.
-
-val GSPEC_PRS = store_thm
-   ("GSPEC_PRS",
-    (--`!R1 (abs1:'a -> 'c) rep1. QUOTIENT R1 abs1 rep1 ==>
-        !R2 (abs2:'b -> 'd) rep2. QUOTIENT R2 abs2 rep2 ==>
-         !f. GSPEC f =
-               SET_MAP rep2 (GSPEC ((abs1 --> (rep2 ## I)) f))`--),
-    REPEAT STRIP_TAC
-    THEN IMP_RES_TAC QUOTIENT_ABS_REP
-    THEN REWRITE_TAC[EXTENSION]
-    THEN GEN_TAC
-    THEN REWRITE_TAC[GSPECIFICATION,IN_SET_MAP]
-    THEN REWRITE_TAC[FUN_MAP_THM,PAIR_MAP]
-    THEN REWRITE_TAC[PAIR_EQ,I_THM]
-    THEN EQ_TAC
-    THEN STRIP_TAC
-    THENL
-      [ EXISTS_TAC ``rep1 (x':'c) :'a``
-        THEN ASM_REWRITE_TAC[]
-        THEN POP_ASSUM (REWRITE_THM o SYM),
-
-        EXISTS_TAC ``abs1 (x':'a) :'c``
-        THEN CONV_TAC (RAND_CONV (REWR_CONV (GSYM PAIR)))
-        THEN REWRITE_TAC[PAIR_EQ]
-        THEN POP_ASSUM REWRITE_THM
-        THEN POP_ASSUM (MP_TAC o AP_TERM ``abs2:'b->'d``)
-        THEN ASM_REWRITE_TAC[]
-      ]
-   );
-
-val GSPECR_def =
-    Define
-      `GSPECR R (f:'a -> ('b # bool)) (v:'b) =
-                     ?x. (R ### $=) (v,T) (f x)`;
-
-
-val GSPECIFICATION_R = store_thm
-   ("GSPECIFICATION_R",
-    (--`!R f v:'b. v IN GSPECR R f = ?x:'a. (R ### $=) (v,T) (f x)`--),
-    REWRITE_TAC[GSPECR_def,SPECIFICATION]
-   );
-
-val GSPECR_PRS = store_thm
-   ("GSPECR_PRS",
-    (--`!R1 (abs1:'a -> 'c) rep1. QUOTIENT R1 abs1 rep1 ==>
-        !R2 (abs2:'b -> 'd) rep2. QUOTIENT R2 abs2 rep2 ==>
-         !f. GSPEC f =
-               SET_MAP rep2 (GSPECR R2 ((abs1 --> (rep2 ## I)) f))`--),
-    REPEAT STRIP_TAC
-    THEN IMP_RES_TAC QUOTIENT_ABS_REP
-    THEN IMP_RES_TAC QUOTIENT_REP_REFL
-    THEN REWRITE_TAC[EXTENSION]
-    THEN GEN_TAC
-    THEN REWRITE_TAC[GSPECIFICATION,GSPECIFICATION_R,IN_SET_MAP]
-    THEN REWRITE_TAC[FUN_MAP_THM,I_THM,PAIR_MAP]
-    THEN REWRITE_TAC[PAIR_REL_THM,PAIR_EQ]
-    THEN EQ_TAC
-    THEN STRIP_TAC
-    THENL
-      [ EXISTS_TAC ``rep1 (x':'c) :'a``
-        THEN ASM_REWRITE_TAC[]
-        THEN POP_ASSUM (REWRITE_THM o SYM)
-        THEN ASM_REWRITE_TAC[],
-
-        EXISTS_TAC ``abs1 (x':'a) :'c``
-        THEN CONV_TAC (RAND_CONV (REWR_CONV (GSYM PAIR)))
-        THEN REWRITE_TAC[PAIR_EQ]
-        THEN POP_ASSUM REWRITE_THM
-        THEN POP_ASSUM MP_TAC
-        THEN IMP_RES_THEN ONCE_REWRITE_THM QUOTIENT_REL
-        THEN ASM_REWRITE_TAC[]
-      ]
-   );
-
-This proof fails for the new quotient relations; not reflexive!
-val GSPECR_RSP = store_thm
-   ("GSPECR_RSP",
-    (--`!R1 (abs1:'a -> 'c) rep1. QUOTIENT R1 abs1 rep1 ==>
-        !R2 (abs2:'b -> 'd) rep2. QUOTIENT R2 abs2 rep2 ==>
-         !f1 f2.
-          (R1 ===> (R2 ### $=)) f1 f2 ==>
-          SET_REL R2 (GSPECR R2 f1) (GSPECR R2 f2)`--),
-    REPEAT GEN_TAC THEN DISCH_TAC
-    THEN REPEAT GEN_TAC THEN DISCH_TAC
-    THEN REPEAT GEN_TAC
-    THEN REWRITE_TAC[FUN_REL]
-    THEN ONCE_REWRITE_TAC[GSYM PAIR]
-    THEN REWRITE_TAC[PAIR_REL_THM]
-    THEN DISCH_TAC
-    THEN REWRITE_TAC[SET_REL]
-    THEN X_GEN_TAC ``z:'b``
-    THEN GEN_TAC
-    THEN DISCH_TAC
-    THEN REWRITE_TAC[GSPECIFICATION_R]
-    THEN ONCE_REWRITE_TAC[GSYM PAIR]
-    THEN REWRITE_TAC[PAIR_REL_THM,PAIR_EQ]
-    THEN EQ_TAC
-    THEN STRIP_TAC
-    THEN EXISTS_TAC ``(rep1:'c->'a) ((abs1:'a->'c) x)``
-    THEN IMP_RES_TAC QUOTIENT_REP_REFL
-    THEN FIRST_ASSUM (ASSUME_TAC o SPEC ``(abs1:'a->'c) x``)
-    THEN RES_TAC
-    THEN POP_TAC
-    THEN POP_TAC
-    THEN POP_ASSUM (REWRITE_THM o SYM)
-    THEN IMP_RES_TAC QUOTIENT_SYM
-    THEN IMP_RES_TAC QUOTIENT_TRANS
-   );
-
-Can't prove this, so can't lift GSPEC.
-
-val GSPEC_RSP = store_thm
-   ("GSPEC_RSP",
-    (--`!R1 (abs1:'a -> 'c) rep1 R2 (abs2:'b -> 'd) rep2.
-         (!a. abs1 (rep1 a) = a) /\ (!r r'. R1 r r' = (abs1 r = abs1 r'))
-         ==>
-         (!a. abs2 (rep2 a) = a) /\ (!r r'. R2 r r' = (abs2 r = abs2 r'))
-         ==>
-         !f1 f2.
-          (R1 ===> (R2 ### $=)) f1 f2 ==>
-          SET_REL R2 (GSPEC f1) (GSPEC f2)`--),
-    REPEAT GEN_TAC
-    THEN STRIP_TAC
-    THEN STRIP_TAC
-    THEN REPEAT GEN_TAC
-    THEN REWRITE_TAC[FUN_REL]
-    THEN ONCE_REWRITE_TAC[GSYM PAIR]
-    THEN REWRITE_TAC[PAIR_REL_THM]
-    THEN DISCH_TAC
-    THEN REWRITE_TAC[SET_REL_EQ]
-    THEN REPEAT STRIP_TAC
-    THEN REWRITE_TAC[GSPECIFICATION]
-    THEN ONCE_REWRITE_TAC[GSYM PAIR]
-    THEN REWRITE_TAC[PAIR_EQ]
-    THEN ???
-   );
-
-No, the GSPEC / GSPECR experiment has not succeeded.
-*)
-
-
-val EMPTY_PRS = store_thm
-   ("EMPTY_PRS",
-    (--`!R (abs:'a -> 'b) rep. QUOTIENT R abs rep ==>
-         (EMPTY = SET_MAP abs EMPTY)`--),
-    REPEAT STRIP_TAC
-    THEN REWRITE_TAC[EXTENSION]
-    THEN REWRITE_TAC[NOT_IN_EMPTY,IN_SET_MAP]
-   );
-
-val EMPTY_RSP = store_thm
-   ("EMPTY_RSP",
-    (--`!R (abs:'a -> 'b) rep. QUOTIENT R abs rep ==>
-         SET_REL R EMPTY EMPTY`--),
-    REPEAT STRIP_TAC
-    THEN REWRITE_TAC[SET_REL]
-    THEN REWRITE_TAC[NOT_IN_EMPTY]
-   );
-
-val UNIV_PRS = store_thm
-   ("UNIV_PRS",
-    (--`!R (abs:'a -> 'b) rep. QUOTIENT R abs rep ==>
-         (UNIV = SET_MAP abs UNIV)`--),
-    REPEAT STRIP_TAC
-    THEN REWRITE_TAC[EXTENSION]
-    THEN REWRITE_TAC[IN_SET_MAP,IN_UNIV]
-   );
-
-val UNIV_RSP = store_thm
-   ("UNIV_RSP",
-    (--`!R (abs:'a -> 'b) rep. QUOTIENT R abs rep ==>
-         SET_REL R UNIV UNIV`--),
-    REPEAT STRIP_TAC
-    THEN REWRITE_TAC[SET_REL]
-    THEN REWRITE_TAC[IN_UNIV]
-   );
-
-
-val UNION_PRS = store_thm
-   ("UNION_PRS",
-    (--`!R (abs:'a -> 'b) rep. QUOTIENT R abs rep ==>
-         !s t. s UNION t =
-               SET_MAP rep (SET_MAP abs s UNION SET_MAP abs t)`--),
-    REPEAT STRIP_TAC
-    THEN PURE_ONCE_REWRITE_TAC[EXTENSION]
-    THEN GEN_TAC
-    THEN PURE_REWRITE_TAC[IN_SET_MAP,IN_UNION]
-    THEN IMP_RES_TAC QUOTIENT_ABS_REP
-    THEN ASM_REWRITE_TAC[]
-   );
-
-val UNION_RSP = store_thm
-   ("UNION_RSP",
-    (--`!R (abs:'a -> 'b) rep. QUOTIENT R abs rep ==>
-         !s1 s2 t1 t2.
-          SET_REL R s1 s2 /\ SET_REL R t1 t2 ==>
-          SET_REL R (s1 UNION t1) (s2 UNION t2)`--),
-    REPEAT STRIP_TAC
-    THEN PURE_REWRITE_TAC[SET_REL]
-    THEN REPEAT STRIP_TAC
-    THEN PURE_REWRITE_TAC[IN_UNION]
-    THEN IMP_RES_TAC (REWRITE_RULE[GSYM AND_IMP_INTRO] SET_REL_MP)
-    THEN ASM_REWRITE_TAC[]
-   );
-
-
-val INTER_PRS = store_thm
-   ("INTER_PRS",
-    (--`!R (abs:'a -> 'b) rep. QUOTIENT R abs rep ==>
-         !s t. s INTER t =
-               SET_MAP rep (SET_MAP abs s INTER SET_MAP abs t)`--),
-    REPEAT STRIP_TAC
-    THEN PURE_ONCE_REWRITE_TAC[EXTENSION]
-    THEN GEN_TAC
-    THEN PURE_REWRITE_TAC[IN_SET_MAP,IN_INTER]
-    THEN IMP_RES_TAC QUOTIENT_ABS_REP
-    THEN ASM_REWRITE_TAC[]
-   );
-
-val INTER_RSP = store_thm
-   ("INTER_RSP",
-    (--`!R (abs:'a -> 'b) rep. QUOTIENT R abs rep ==>
-         !s1 s2 t1 t2.
-          SET_REL R s1 s2 /\ SET_REL R t1 t2 ==>
-          SET_REL R (s1 INTER t1) (s2 INTER t2)`--),
-    REPEAT STRIP_TAC
-    THEN PURE_REWRITE_TAC[SET_REL]
-    THEN REPEAT STRIP_TAC
-    THEN PURE_REWRITE_TAC[IN_INTER]
-    THEN IMP_RES_TAC (REWRITE_RULE[GSYM AND_IMP_INTRO] SET_REL_MP)
-    THEN ASM_REWRITE_TAC[]
-   );
-
-(*
-val EQ_EMPTY_PRS = store_thm
-   ("EQ_EMPTY_PRS",
-    (--`!R (abs:'a -> 'b) rep. QUOTIENT R abs rep ==>
-         !s.
-             (s = {}) = (SET_MAP abs s = {})`--),
-    REPEAT STRIP_TAC
-    THEN REWRITE_TAC[EXTENSION,NOT_IN_EMPTY]
-    THEN REWRITE_TAC[IN_SET_MAP]
-    THEN EQ_TAC
-    THENL
-      [ DISCH_TAC
-        THEN GEN_TAC
-        THEN POP_ASSUM MATCH_ACCEPT_TAC,
-
-        DISCH_TAC
-        THEN GEN_TAC
-        THEN POP_ASSUM (MP_TAC o SPEC ``rep (x:'b) :'a``)
-        THEN IMP_RES_TAC QUOTIENT_ABS_REP
-        THEN ASM_REWRITE_TAC[]
-      ]
-   );
-
-val EQ_EMPTY_RSP = store_thm
-   ("EQ_EMPTY_RSP",
-    (--`!R (abs:'a -> 'b) rep. QUOTIENT R abs rep ==>
-         !s1 s2. SET_REL R s1 s2 ==>
-             ((s1 = {}) = (s2 = {}))`--),
-    REWRITE_TAC[SET_REL]
-    THEN REPEAT STRIP_TAC
-    THEN REWRITE_TAC[EXTENSION,NOT_IN_EMPTY]
-    THEN EQ_TAC
-    THENL
-      [ DISCH_TAC
-        THEN GEN_TAC
-        THEN POP_ASSUM MATCH_ACCEPT_TAC,
-
-        DISCH_TAC
-        THEN GEN_TAC
-        THEN POP_ASSUM (MP_TAC o SPEC ``rep (x:'b) :'a``)
-        THEN IMP_RES_TAC QUOTIENT_ABS_REP
-        THEN ASM_REWRITE_TAC[]
-      ]
-   );
-*)
-
-(* DISJOINT does not lift.
-
-val DISJOINTR_def =
-    Define
-      `DISJOINTR R (s:'a -> bool) t = SET_REL R (s INTER t) {}`;
-
-NO.
-val SET_REL_EXTENSION = store_thm
-   ("SET_REL_EXTENSION",
-    (--`!R (abs:'a -> 'b) rep. QUOTIENT R abs rep ==>
-         !s t. SET_REL R s t = (!x :: respects R. x IN s = x IN t)`--),
-    REPEAT STRIP_TAC
-    THEN REWRITE_TAC[SET_REL]
-    THEN CONV_TAC (DEPTH_CONV RES_FORALL_CONV)
-    THEN REWRITE_TAC[IN_RESPECTS]
-    THEN EQ_TAC
-    THENL
-      [ DISCH_TAC
-        THEN GEN_TAC
-        THEN POP_ASSUM MATCH_ACCEPT_TAC,
-
-        DISCH_TAC
-        THEN REPEAT GEN_TAC
-        THEN POP_ASSUM (MP_TAC o SPEC ``rep (x:'b) :'a``)
-        THEN IMP_RES_TAC QUOTIENT_REP_REFL
-        THEN ASM_REWRITE_TAC[]
-      ]
-   );
-
-val DISJOINT_PRS = store_thm
-   ("DISJOINT_PRS",
-    (--`!R (abs:'a -> 'b) rep. QUOTIENT R abs rep ==>
-         !s t.
-             DISJOINT s t = DISJOINTR R (SET_MAP abs s) (SET_MAP abs t)`--),
-    REPEAT STRIP_TAC
-    THEN PURE_REWRITE_TAC[DISJOINT_DEF,DISJOINTR_def]
-    THEN REWRITE_TAC[EXTENSION,NOT_IN_EMPTY,IN_INTER]
-    THEN REWRITE_TAC[SET_REL_EXTENSION,NOT_IN_EMPTY,IN_INTER]
-    THEN REWRITE_TAC[IN_SET_MAP]
-    THEN EQ_TAC
-    THENL
-      [ DISCH_TAC
-        THEN GEN_TAC
-        THEN POP_ASSUM MATCH_ACCEPT_TAC,
-
-        DISCH_TAC
-        THEN GEN_TAC
-        THEN POP_ASSUM (MP_TAC o SPEC ``rep (x:'b) :'a``)
-        THEN IMP_RES_TAC QUOTIENT_ABS_REP
-        THEN ASM_REWRITE_TAC[]
-      ]
-   );
-
-val DISJOINT_RSP = store_thm
-   ("DISJOINT_RSP",
-    (--`!R (abs:'a -> 'b) rep. QUOTIENT R abs rep ==>
-         !s1 s2 t1 t2.
-          SET_REL R s1 s2 /\ SET_REL R t1 t2 ==>
-          (DISJOINT s1 t1 = DISJOINT s2 t2)`--),
-    REPEAT STRIP_TAC
-    THEN PURE_REWRITE_TAC[DISJOINT_DEF]
-    THEN AP_THM_TAC
-    THEN AP_TERM_TAC
-    THEN MP_TAC (SPEC_ALL INTER_RSP)
-    THEN ASM_REWRITE_TAC[]
-    THEN 
-    THEN 
-    THEN 
-    THEN IMP_RES_THEN MATCH_MP_TAC INTER_RSP
-    THEN 
-    THEN REWRITE_TAC[EXTENSION,NOT_IN_EMPTY,IN_INTER]
-    THEN REWRITE_TAC[DE_MORGAN_THM]
-    THEN EQ_TAC
-    THEN DISCH_TAC
-    THEN GEN_TAC
-    THEN POP_ASSUM (MP_TAC o SPEC ``x:'a``)
-    THEN IMP_RES_TAC QUOTIENT_REFL
-    THEN POP_ASSUM (ASSUME_TAC o SPEC ``x:'a``)
-    THEN IMP_RES_TAC SET_REL_MP
-    THEN ASM_REWRITE_TAC[]
-   );
-*)
-
-
-
-val SUBSETR_def =
-    Define
-      `SUBSETR P s t = !x:'a::P. x IN s ==> x IN t`;
-
-val SUBSET_PRS = store_thm
-   ("SUBSET_PRS",
-    (--`!R (abs:'a -> 'b) rep. QUOTIENT R abs rep ==>
-         !s t. s SUBSET t =
-               SUBSETR (respects R) (SET_MAP abs s) (SET_MAP abs t)`--),
-    REPEAT STRIP_TAC
-    THEN PURE_REWRITE_TAC[SUBSET_DEF,SUBSETR_def]
-    THEN PURE_REWRITE_TAC[IN_SET_MAP]
-    THEN CONV_TAC (RAND_CONV RES_FORALL_CONV)
-    THEN PURE_REWRITE_TAC[IN_RESPECTS]
-    THEN EQ_TAC
-    THEN DISCH_TAC
-    THEN GEN_TAC
-    THENL
-      [ DISCH_TAC
-        THEN FIRST_ASSUM MATCH_ACCEPT_TAC,
-
-        POP_ASSUM (MP_TAC o SPEC ``rep (x:'b) :'a``)
-        THEN IMP_RES_TAC QUOTIENT_ABS_REP
-        THEN IMP_RES_TAC QUOTIENT_REP_REFL
-        THEN ASM_REWRITE_TAC[]
-      ]
-   );
-
-val SUBSETR_RSP = store_thm
-   ("SUBSETR_RSP",
-    (--`!R (abs:'a -> 'b) rep. QUOTIENT R abs rep ==>
-         !s1 s2 t1 t2.
-          SET_REL R s1 s2 /\ SET_REL R t1 t2 ==>
-          (SUBSETR (respects R) s1 t1 = SUBSETR (respects R) s2 t2)`--),
-    REPEAT GEN_TAC THEN DISCH_TAC
-    THEN REPEAT GEN_TAC
-    THEN REWRITE_TAC[SET_REL]
-    THEN STRIP_TAC
-    THEN PURE_REWRITE_TAC[SUBSETR_def]
-    THEN CONV_TAC (DEPTH_CONV RES_FORALL_CONV)
-    THEN PURE_REWRITE_TAC[IN_RESPECTS]
-    THEN EQ_TAC
-    THEN DISCH_TAC
-    THEN GEN_TAC
-    THEN DISCH_TAC
-    THEN DISCH_TAC
-    THEN RES_TAC
-    THEN RES_TAC
-   );
-
-
-val PSUBSETR_def =
-    Define
-      `PSUBSETR R (s:'a->bool) t =
-       SUBSETR (respects R) s t /\ ~(SET_REL R s t)`;
-
-val PSUBSET_PRS = store_thm
-   ("PSUBSET_PRS",
-    (--`!R (abs:'a -> 'b) rep. QUOTIENT R abs rep ==>
-         !s t. s PSUBSET t = PSUBSETR R (SET_MAP abs s) (SET_MAP abs t)`--),
-    REPEAT STRIP_TAC
-    THEN PURE_REWRITE_TAC[PSUBSET_DEF,PSUBSETR_def]
-    THEN PURE_ONCE_REWRITE_TAC[EXTENSION]
-    THEN PURE_ONCE_REWRITE_TAC[SET_REL]
-    THEN PURE_REWRITE_TAC[IN_SET_MAP]
-    THEN IMP_RES_THEN REWRITE_THM SUBSET_PRS
-    THEN AP_TERM_TAC
-    THEN AP_TERM_TAC
-    THEN EQ_TAC
-    THEN REPEAT STRIP_TAC
-    THENL
-      [ IMP_RES_TAC QUOTIENT_REL_ABS
-        THEN ASM_REWRITE_TAC[],
-
-        IMP_RES_THEN (ASSUME_TAC o SPEC ``x:'b``) QUOTIENT_REP_REFL
-        THEN RES_THEN MP_TAC
-        THEN IMP_RES_THEN REWRITE_THM QUOTIENT_ABS_REP
-      ]
-   );
-
-val PSUBSETR_RSP = store_thm
-   ("PSUBSETR_RSP",
-    (--`!R (abs:'a -> 'b) rep. QUOTIENT R abs rep ==>
-         !s1 s2 t1 t2.
-          SET_REL R s1 s2 /\ SET_REL R t1 t2 ==>
-          (PSUBSETR R s1 t1 = PSUBSETR R s2 t2)`--),
-    REPEAT STRIP_TAC
-    THEN PURE_REWRITE_TAC[PSUBSETR_def]
-    THEN MP_TAC (SPEC_ALL SUBSETR_RSP)
-    THEN ASM_REWRITE_TAC[]
-    THEN DISCH_THEN (MP_TAC o SPEC_ALL)
-    THEN ASM_REWRITE_TAC[]
-    THEN DISCH_THEN REWRITE_THM
-    THEN AP_TERM_TAC
-    THEN AP_TERM_TAC
-    THEN IMP_RES_TAC SET_QUOTIENT
-    THEN POP_ASSUM (MATCH_MP_TAC o (MATCH_MP EQUALS_RSP))
-    THEN ASM_REWRITE_TAC[]
-   );
-
-
-(* IMAGER (rep1,abs2) f s =
-   SET_MAP abs2 (IMAGE ((rep1 --> abs2) f) (SET_MAP rep1 s))
-
-   SET_MAP abs2 {(rep1 --> abs2) f x | x IN SET_MAP rep1 s}
-
-   SET_MAP abs2 {(rep1 --> abs2) f x | rep1 x IN s}
-
-   SET_MAP abs2 {abs2 (f (rep1 x)) | rep1 x IN s}
-
-   SET_MAP abs2 {abs2 (f z) | R1 z z /\ z IN s}
-
-   SET_MAP abs2 {abs2 (f z) | R1 z z /\ z IN s}
-
-   {y | ?x. abs2 y = abs2 (f x) /\ R1 x x /\ x IN s}
-
-   {y | ?x. R2 y (f x) /\ R1 x x /\ x IN s}
-
-?  {y | ?x. R2 y (f (rep1 x)) /\ rep1 x IN s}
-
-?  {y | ?x x'. R2 y (f x) /\ R1 x x' /\ x' IN s}
-
-  *)
-
-(*
-val IMAGER_def =
-    Define
-      `IMAGER R1 R2 (f:'a->'b) s =
-       {y:'b | ?x :: respects R1. R2 y (f x) /\ x IN s}`;
-*)
-
-val IMAGER_def =
-    Define
-      `IMAGER R1 R2 (f:'a->'b) s =
-       {y:'b | ?x :: respects R1. R2 y (f x) /\ x IN s}`;
-
-val IN_IMAGER = store_thm
-   ("IN_IMAGER",
-    (--`!R1 R2 y (f:'a -> 'b) s.
-          y IN IMAGER R1 R2 f s =
-                 ?x :: respects R1. R2 y (f x) /\ x IN s`--),
-    REPEAT GEN_TAC
-    THEN PURE_ONCE_REWRITE_TAC[IMAGER_def]
-    THEN CONV_TAC (DEPTH_CONV pred_setLib.SET_SPEC_CONV)
-    THEN REWRITE_TAC[]
-   );
-
-val IMAGE_PRS = store_thm
-   ("IMAGE_PRS",
-    (--`!R1 (abs1:'a -> 'c) rep1. QUOTIENT R1 abs1 rep1 ==>
-        !R2 (abs2:'b -> 'd) rep2. QUOTIENT R2 abs2 rep2 ==>
-         !f s. IMAGE f s =
-               SET_MAP rep2 (IMAGER R1 R2 ((abs1-->rep2) f) (SET_MAP abs1 s))
-       `--),
-    REPEAT STRIP_TAC
-    THEN IMP_RES_TAC QUOTIENT_ABS_REP
-    THEN PURE_ONCE_REWRITE_TAC[EXTENSION]
-    THEN GEN_TAC
-    THEN PURE_REWRITE_TAC[IN_SET_MAP,IN_IMAGE,IN_IMAGER]
-    THEN CONV_TAC (DEPTH_CONV RES_EXISTS_CONV)
-    THEN REWRITE_TAC[IN_RESPECTS,FUN_MAP_THM]
-    THEN EQ_TAC
-    THENL
-       [ STRIP_TAC
-         THEN EXISTS_TAC (--`(rep1:'c->'a) x'`--)
-         THEN IMP_RES_TAC QUOTIENT_REP_REFL
-         THEN ASM_REWRITE_TAC[],
-
-         STRIP_TAC
-         THEN EXISTS_TAC (--`(abs1:'a->'c) x'`--)
-         THEN POP_ASSUM (fn th => REWRITE_TAC[th])
-         THEN IMP_RES_TAC QUOTIENT_REL_ABS
-         THEN POP_TAC
-         THEN POP_ASSUM MP_TAC
-         THEN ASM_REWRITE_TAC[]
-       ]
-   );
-
-val IMAGER_RSP = store_thm
-   ("IMAGER_RSP",
-    (--`!R1 (abs1:'a -> 'c) rep1. QUOTIENT R1 abs1 rep1 ==>
-        !R2 (abs2:'b -> 'd) rep2. QUOTIENT R2 abs2 rep2 ==>
-         !f1 f2 s1 s2.
-          (R1 ===> R2) f1 f2 /\ SET_REL R1 s1 s2 ==>
-          SET_REL R2 (IMAGER R1 R2 f1 s1) (IMAGER R1 R2 f2 s2)`--),
-    REPEAT GEN_TAC
-    THEN STRIP_TAC
-    THEN REPEAT GEN_TAC
-    THEN STRIP_TAC
-    THEN REPEAT GEN_TAC
-    THEN REWRITE_TAC[SET_REL]
-    THEN REWRITE_TAC[FUN_REL]
-    THEN REPEAT STRIP_TAC
-    THEN REWRITE_TAC[IN_IMAGER]
-    THEN CONV_TAC (DEPTH_CONV RES_EXISTS_CONV)
-    THEN REWRITE_TAC[IN_RESPECTS]
-    THEN EQ_TAC
-    THEN STRIP_TAC
-    THEN EXISTS_TAC (--`x':'a`--)
-    THEN RES_TAC
-    THEN ASM_REWRITE_TAC[]
-    THEN IMP_RES_TAC QUOTIENT_SYM
-    THEN IMP_RES_TAC QUOTIENT_TRANS
-   );
-
-(*
-val IMAGE_RSP = store_thm
-   ("IMAGE_RSP",
-    (--`!R1 (abs1:'a -> 'c) rep1. QUOTIENT R1 abs1 rep1 ==>
-        !R2 (abs2:'b -> 'd) rep2. QUOTIENT R2 abs2 rep2 ==>
-         !f1 f2 s1 s2.
-          (R1 ===> R2) f1 f2 /\ SET_REL R1 s1 s2 ==>
-          SET_REL R2 (IMAGE f1 s1) (IMAGE f2 s2)`--),
-    REPEAT GEN_TAC THEN DISCH_TAC
-    THEN REPEAT GEN_TAC THEN DISCH_TAC
-    THEN REPEAT GEN_TAC
-    THEN REWRITE_TAC[FUN_REL,SET_REL]
-    THEN REPEAT STRIP_TAC
-    THEN REWRITE_TAC[IN_IMAGE]
-    THEN EQ_TAC
-    THEN STRIP_TAC
-    THENL
-       [ EXISTS_TAC (--`x':'a`--)
-         THEN CONJ_TAC
-         THENL
-           [ ASM_REWRITE_TAC[]
-             THEN FIRST_ASSUM MATCH_MP_TAC
-             THEN ASM_REWRITE_TAC[],
-
-             POP_ASSUM MP_TAC
-             THEN ASM_REWRITE_TAC[]
-           ],
-
-         EXISTS_TAC (--`x':'a`--)
-         THEN CONJ_TAC
-         THENL
-           [ ASM_REWRITE_TAC[]
-             THEN ONCE_REWRITE_TAC[EQ_SYM_EQ]
-             THEN FIRST_ASSUM MATCH_MP_TAC
-             THEN ASM_REWRITE_TAC[],
-
-             POP_ASSUM MP_TAC
-             THEN ASM_REWRITE_TAC[]
-           ]
-       ]
-   );
-*)
-
-
-
-
 (* ----------------------------------------- *)
 (* theorems for regularized version of goals *)
 (* ----------------------------------------- *)
@@ -2201,10 +1420,11 @@ val NOT_IMPLIES = store_thm
 val EQUALS_EQUIV_IMPLIES = store_thm
    ("EQUALS_EQUIV_IMPLIES",
     (--`!R:'a -> 'a -> bool.
-          (!x y. R x y = (R x = R y)) ==>
+          EQUIV R  ==>
           R a1 a2 /\ R b1 b2 ==>
           ((a1 = b1) ==> R a2 b2)`--),
-    REPEAT STRIP_TAC
+    REWRITE_TAC[EQUIV_def]
+    THEN REPEAT STRIP_TAC
     THEN POP_ASSUM REWRITE_ALL_THM
     THEN IMP_RES_TAC EQUIV_REFL_SYM_TRANS
    );
@@ -2213,10 +1433,11 @@ val EQUALS_EQUIV_IMPLIES = store_thm
 val EQUALS_EQUIV_IMPLIES1 = store_thm
    ("EQUALS_EQUIV_IMPLIES1",
     (--`!R:'a -> 'a -> bool.
-          (!x y. R x y = (R x = R y)) ==>
+          EQUIV R  ==>
           (R a1 b1 ==> R a2 b2) ==>
           ((a1 = b1) ==> R a2 b2)`--),
-    REPEAT STRIP_TAC
+    REWRITE_TAC[EQUIV_def]
+    THEN REPEAT STRIP_TAC
     THEN POP_ASSUM REWRITE_ALL_THM
     THEN FIRST_ASSUM MATCH_MP_TAC
     THEN ASM_REWRITE_TAC[]
@@ -2280,9 +1501,10 @@ val EQUIV_RES_ABSTRACT_RIGHT = store_thm
 val EQUIV_RES_FORALL = store_thm
    ("EQUIV_RES_FORALL",
     (--`!E (P:'a -> bool).
-          (!x y. E x y = (E x = E y)) ==>
+          EQUIV E ==>
           (RES_FORALL (respects E) P = ($! P))`--),
-    REPEAT STRIP_TAC
+    REWRITE_TAC[EQUIV_def]
+    THEN REPEAT STRIP_TAC
     THEN CONV_TAC (LAND_CONV (RAND_CONV (REWR_CONV (GSYM ETA_AX))))
     THEN CONV_TAC (RAND_CONV (RAND_CONV (REWR_CONV (GSYM ETA_AX))))
     THEN CONV_TAC (LAND_CONV res_quanLib.RES_FORALL_CONV)
@@ -2292,9 +1514,10 @@ val EQUIV_RES_FORALL = store_thm
 val EQUIV_RES_EXISTS = store_thm
    ("EQUIV_RES_EXISTS",
     (--`!E (P:'a -> bool).
-          (!x y. E x y = (E x = E y)) ==>
+          EQUIV E ==>
           (RES_EXISTS (respects E) P = ($? P))`--),
-    REPEAT STRIP_TAC
+    REWRITE_TAC[EQUIV_def]
+    THEN REPEAT STRIP_TAC
     THEN CONV_TAC (LAND_CONV (RAND_CONV (REWR_CONV (GSYM ETA_AX))))
     THEN CONV_TAC (RAND_CONV (RAND_CONV (REWR_CONV (GSYM ETA_AX))))
     THEN CONV_TAC (LAND_CONV res_quanLib.RES_EXISTS_CONV)
@@ -2304,9 +1527,10 @@ val EQUIV_RES_EXISTS = store_thm
 val EQUIV_RES_EXISTS_UNIQUE = store_thm
    ("EQUIV_RES_EXISTS_UNIQUE",
     (--`!E (P:'a -> bool).
-          (!x y. E x y = (E x = E y)) ==>
+          EQUIV E ==>
           (RES_EXISTS_UNIQUE (respects E) P = ($?! P))`--),
-    REPEAT STRIP_TAC
+    REWRITE_TAC[EQUIV_def]
+    THEN REPEAT STRIP_TAC
     THEN CONV_TAC (LAND_CONV (RAND_CONV (REWR_CONV (GSYM ETA_AX))))
     THEN CONV_TAC (RAND_CONV (RAND_CONV (REWR_CONV (GSYM ETA_AX))))
     THEN CONV_TAC (LAND_CONV res_quanLib.RES_EXISTS_UNIQUE_CONV)
