src/quotient/examples/finite_setScript.sml
@@ -1,0 +1,767 @@
+open HolKernel Parse boolLib;
+infix THEN THENL THENC ORELSE ORELSEC THEN_TCL ORELSE_TCL ## |->;
+infixr -->;
+
+
+(* ------------------------------------------------------------------------ *)
+(* Representing finite sets as a new datatype in the HOL logic.             *)
+(*                                                                          *)
+(* This is a demonstration of how to use the higher order quotient package  *)
+(* to construct the type of finite sets, modeled as a quotient of lists.    *)
+(* ------------------------------------------------------------------------ *)
+
+
+val _ = new_theory "finite_set";
+
+
+(* In interactive sessions, do:
+
+app load ["listTheory",
+          "pred_setTheory",
+          "ind_rel",
+          "bossLib",
+          "quotientLib"];
+
+*)
+
+open listTheory;
+open pred_setTheory;
+open ind_rel;
+open bossLib;
+
+open quotientLib;
+
+
+val REWRITE_THM = fn th => REWRITE_TAC[th];
+
+
+(* --------------------------------------------------------------------- *)
+(* Section 1, The Concrete Datatype and the Equivalence Relation.        *)
+(* --------------------------------------------------------------------- *)
+
+(* --------------------------------------------------------------------- *)
+(* Use finite lists for the free algebra of {{},INSERT} finite sets.     *)
+(* --------------------------------------------------------------------- *)
+
+
+(* --------------------------------------------------------------------- *)
+(* Definition of equivalence between lists as finite sets.               *)
+(* This uses Myra VanInwegen's mutually recursive rule induction pkg.    *)
+(* See ind_rel.sig and ind_rel.sml.                                      *)
+(* --------------------------------------------------------------------- *)
+
+
+val fsequiv = --`fsequiv: 'a list -> 'a list -> bool`--;
+
+val fsequiv_patterns = [--`^fsequiv S1 S2`--];
+
+val fsequiv_rules_tm =
+--`
+
+
+       (* ------------------------------------------------------ *)
+               (^fsequiv (a :: (b :: A)) (b :: (a :: A)))               /\
+
+
+       (* ------------------------------------------------------ *)
+                  (^fsequiv (a :: (a :: A)) (a :: A))                   /\
+
+
+                      
+       (* ------------------------------------------------------ *)
+                           (^fsequiv [] [])                             /\
+
+
+                           ((^fsequiv A B)
+       (* ------------------------------------------------------ *) ==>
+                     (^fsequiv (a :: A) (a :: B)))                      /\
+
+
+                           ((^fsequiv A B)
+       (* ------------------------------------------------------ *) ==>
+                            (^fsequiv B A))                             /\
+
+
+                    ((^fsequiv A B) /\ (^fsequiv B C)
+       (* ------------------------------------------------------ *) ==>
+                            (^fsequiv A C))                      
+
+`--;
+
+val (fsequiv_rules_sat,fsequiv_ind_thm) =
+    define_inductive_relations fsequiv_patterns fsequiv_rules_tm;
+
+val fsequiv_inv_thms = prove_inversion_theorems
+    fsequiv_rules_sat fsequiv_ind_thm;
+
+val fsequiv_strong_ind = prove_strong_induction 
+    fsequiv_rules_sat fsequiv_ind_thm;
+
+val _ = overload_on("==", ``fsequiv:'a list -> 'a list -> bool``);
+val _ = add_infix ("==", 425, HOLgrammars.NONASSOC);
+
+val _ = save_thm ("fsequiv_rules_sat", fsequiv_rules_sat);
+val _ = save_thm ("fsequiv_ind_thm", fsequiv_ind_thm);
+val _ = save_thm ("fsequiv_inv_thms", LIST_CONJ fsequiv_inv_thms);
+val _ = save_thm ("fsequiv_strong_ind", fsequiv_strong_ind);
+
+
+val [CONS_LEFT_COMM, CONS_LEFT_IDEM, NIL_RSP, CONS_RSP, fset_SYM', fset_TRANS']
+    = CONJUNCTS fsequiv_rules_sat;
+
+
+(* The finite set equivalence relation is reflexive, symmetric and transitive.*)
+
+val fset_REFL = store_thm
+   ("fset_REFL",
+    ``!X:'a list. X == X``,
+    Induct
+    THEN RW_TAC std_ss [fsequiv_rules_sat]
+   );
+
+val fset_SYM = store_thm
+   ("fset_SYM",
+    ``!X Y:'a list.
+           X == Y ==> Y == X``,
+    REWRITE_TAC [fset_SYM']
+   );
+
+val fset_TRANS = store_thm
+   ("fset_TRANS",
+    ``!X Y Z:'a list.
+           X == Y /\ Y == Z ==> X == Z``,
+    PROVE_TAC [fset_TRANS']
+   );
+
+val fset_NIL = store_thm
+   ("fset_NIL",
+    ``!A B:'a list.
+           A == B ==> ((A = []) = (B = []))``,
+    rule_induct fsequiv_ind_thm
+    THEN REPEAT STRIP_TAC
+    THEN RW_TAC list_ss []
+   );
+
+
+
+(* --------------------------------------------------------------------- *)
+(* Section 2, Functions on the Free Algebra.                             *)
+(*                                                                       *)
+(* We either use as predefined, or define new here, the following        *)
+(* functions:                                                            *)
+(*                                                                       *)
+(*     MEM       test of membership of an element in a list              *)
+(*     Card1     number of distinct elements in a list                   *)
+(*     Delete1   delete all instances of an element from a list          *)
+(*     APPEND    concatenate two lists                                   *)
+(*     Inter1    intersection of two lists                               *)
+(*     Fold1     computes the fold of a function on a list               *)
+(*     list2set  conversion of a list into a set                         *)
+(*                                                                       *)
+(* For each such function its respectfulness theorem is proven.          *)
+(* --------------------------------------------------------------------- *)
+
+(* --------------------------------------------------------------------- *)
+(* The membership function to test if an element is a member of a list   *)
+(* is predefined in the list library as MEM:                             *)
+(*                                                                       *)
+(*    |- (!x. MEM x [] = F) /\                                           *)
+(*       (!x h t. MEM x (h::t) = (x = h) \/ MEM x t)                     *)
+(* --------------------------------------------------------------------- *)
+
+val _ = overload_on("MEM", ``MEM :'a -> 'a list -> bool``);
+
+val MEM_RSP1 = store_thm
+   ("MEM_RSP1",
+    ``!X Y. X == Y ==> (!x:'a. MEM x X = MEM x Y)``,
+    rule_induct fsequiv_ind_thm
+    THEN REPEAT STRIP_TAC
+    THEN RW_TAC std_ss [MEM]
+    THEN PROVE_TAC []
+   );
+
+val MEM_RSP = store_thm
+   ("MEM_RSP",
+    ``!X Y (x:'a). X == Y ==> (MEM x X = MEM x Y)``,
+    PROVE_TAC [MEM_RSP1]
+   );
+
+val NO_MEM_NIL = store_thm
+   ("NO_MEM_NIL",
+    ``!A. (!a:'a. ~(MEM a A)) = (A = [])``,
+    Induct
+    THEN RW_TAC std_ss [MEM]
+    THEN PROVE_TAC [fsequiv_rules_sat]
+   );
+
+val NONE_MEM_NIL = store_thm
+   ("NONE_MEM_NIL",
+    ``!A. (!a:'a. ~(MEM a A)) = (A == [])``,
+    REWRITE_TAC [NO_MEM_NIL]
+    THEN PROVE_TAC [fsequiv_rules_sat,fset_NIL]
+   );
+
+val MEM_CONS = store_thm
+   ("MEM_CONS",
+    ``!A (a:'a). MEM a A ==> (a :: A) == A``,
+    Induct
+    THEN RW_TAC std_ss [MEM]
+    THEN PROVE_TAC [fsequiv_rules_sat]
+   );
+
+val finite_set1_strong_cases = store_thm
+   ("finite_set1_strong_cases",
+    ``!X. (X = []) \/ ?(a:'a) Y. ~(MEM a Y) /\ X == (a :: Y)``,
+    Induct
+    THEN PROVE_TAC [MEM,MEM_CONS,fsequiv_rules_sat]
+   );
+
+(* --------------------------------------------------------------------- *)
+(* Definition of Card function to measure the size of a finite set.      *)
+(* --------------------------------------------------------------------- *)
+
+val Card1_def = Define
+   `(Card1 ([]) = 0)  /\
+    (Card1 ((a:'a) :: A) = if MEM a A then Card1 A else SUC (Card1 A))`;
+
+val Card1_RSP = store_thm
+   ("Card1_RSP",
+    ``!A B:'a list. A == B ==> (Card1 A = Card1 B)``,
+    rule_induct fsequiv_strong_ind
+    THEN REPEAT STRIP_TAC
+    THEN RW_TAC arith_ss [Card1_def,MEM]
+    THEN PROVE_TAC [MEM_RSP]
+   );
+
+val Card1_0 = store_thm
+   ("Card1_0",
+    ``!A:'a list. (Card1 A = 0) = (A = [])``,
+    Induct
+    THEN RW_TAC std_ss [Card1_def]
+    THEN PROVE_TAC[NO_MEM_NIL]
+   );
+
+val NOT_MEM_Card1 = store_thm
+   ("NOT_MEM_Card1",
+    ``!A:'a list a. ~(MEM a A) ==>
+             (Card1 (a :: A) = SUC (Card1 A))``,
+    RW_TAC std_ss [Card1_def]
+   );
+
+val Card1_SUC = store_thm
+   ("Card1_SUC",
+    ``!A n. (Card1 A = SUC n) ==>
+          (?(a:'a) B. ~(MEM a B) /\ A == (a :: B))``,
+    Induct
+    THEN RW_TAC std_ss [Card1_def]
+    THENL
+      [ PROVE_TAC[MEM_CONS,fsequiv_rules_sat],
+
+        PROVE_TAC[fset_REFL]
+      ]
+   );
+
+val Card1_CONS_GT_0 = store_thm
+   ("Card1_CONS_GT_0",
+    ``!A (a:'a).
+          0 < Card1 (a :: A)``,
+    Induct
+    THEN RW_TAC arith_ss [MEM,Card1_def]
+    THEN PROVE_TAC[MEM_CONS,Card1_RSP]
+   );
+
+val MEM_Card1_NOT_0 = store_thm
+   ("MEM_Card1_NOT_0",
+    ``!A (a:'a).
+         MEM a A ==> ~(Card1 A = 0)``,
+    REPEAT GEN_TAC THEN DISCH_TAC
+    THEN IMP_RES_TAC MEM_CONS
+    THEN IMP_RES_TAC Card1_RSP
+    THEN PROVE_TAC [Card1_CONS_GT_0,prim_recTheory.LESS_NOT_EQ]
+   );
+
+val Card1_SUC_MEM = store_thm
+   ("Card1_SUC_MEM",
+    ``!A. (Card1 A = SUC n) ==> ?a:'a. MEM a A``,
+    Cases
+    THEN PROVE_TAC [Card1_def,MEM,numTheory.NOT_SUC]
+   );
+
+val NOT_NIL_EQUIV_CONS = store_thm
+   ("NOT_NIL_EQUIV_CONS",
+    ``!A (a:'a).
+           ~([] == a :: A)``,
+    REPEAT STRIP_TAC
+    THEN IMP_RES_THEN MP_TAC Card1_RSP
+    THEN RW_TAC arith_ss [Card1_def]
+    THEN IMP_RES_THEN (ACCEPT_TAC o GSYM) MEM_Card1_NOT_0
+   );
+
+(* --------------------------------------------------------------------- *)
+(* Definition of function to delete an element from a finite set;        *)
+(* if the element is not a member then the set is unchanged.             *)
+(* --------------------------------------------------------------------- *)
+
+val Delete1_def = Define
+   `($Delete1 ([]) x = [])  /\
+    ($Delete1 ((a:'a) :: A) x = if a = x then $Delete1 A x
+                                     else a :: ($Delete1 A x))`;
+
+val _ = add_infix ("Delete1", 500, HOLgrammars.LEFT);
+
+val MEM_Delete1 = store_thm
+   ("MEM_Delete1",
+    ``!A (a:'a) x.
+         (MEM x (A Delete1 a)) = ((MEM x A) /\ ~(x = a))``,
+    Induct
+    THEN RW_TAC std_ss [MEM,Delete1_def]
+    THEN PROVE_TAC []
+   );
+
+val MEM_Delete1_IDENT = store_thm
+   ("MEM_Delete1_IDENT",
+    ``!A (a:'a).
+         ~(MEM a (A Delete1 a))``,
+    REWRITE_TAC [MEM_Delete1]
+   );
+
+val Card1_Delete1 = store_thm
+   ("Card1_Delete1",
+    ``!A (a:'a).
+         (Card1 (A Delete1 a) = if MEM a A then Card1 A - 1 else Card1 A)``,
+    Induct
+    THEN RW_TAC arith_ss [MEM, Card1_def, Delete1_def, MEM_Delete1]
+    THEN PROVE_TAC [MEM_Card1_NOT_0,
+                    numLib.ARITH_PROVE ``~(n = 0) ==> (SUC (n - 1) = n)``]
+   );
+
+val CONS_Delete1 = store_thm
+   ("CONS_Delete1",
+    ``!A (a:'a).
+         (a :: (A Delete1 a)) ==
+                  (if MEM a A then A else a :: A)``,
+    Induct
+    THEN RW_TAC std_ss [MEM, Delete1_def]
+    THEN PROVE_TAC [MEM, Delete1_def, fsequiv_rules_sat]
+   );
+
+val MEM_CONS_Delete1 = store_thm
+   ("MEM_CONS_Delete1",
+    ``!A (a:'a). MEM a A ==>
+         (a :: (A Delete1 a)) == A``,
+    PROVE_TAC [CONS_Delete1]
+   );
+
+val finite_set1_Delete1_cases1 = store_thm
+   ("finite_set1_Delete1_cases1",
+    ``!X. (X = []) \/ ?a:'a. X == a :: (X Delete1 a)``,
+    Induct
+    THEN PROVE_TAC [Delete1_def,CONS_Delete1,fsequiv_rules_sat]
+   );
+
+val finite_set1_Delete1_cases = store_thm
+   ("finite_set1_Delete1_cases",
+    ``!X. (X = []) \/
+            ?a:'a. MEM a X /\ X == a :: (X Delete1 a)``,
+    PROVE_TAC[finite_set1_Delete1_cases1,MEM,MEM_RSP]
+   );
+
+(* The following theorem is the most critical and difficult theorem. *)
+
+val list_EXTENSION1 = store_thm
+   ("list_EXTENSION1",
+    ``!n A B.
+         (Card1 A = n) /\
+         (!x:'a. MEM x A = MEM x B) ==>
+         A == B``,
+    Induct
+    THEN REPEAT GEN_TAC
+    THENL
+      [ PROVE_TAC [NO_MEM_NIL,MEM_Card1_NOT_0,fset_REFL],
+
+        STRIP_TAC
+        THEN IMP_RES_TAC Card1_SUC_MEM  (* Chooses element "a" of list "A" *)
+        THEN FIRST_ASSUM (C UNDISCH_THEN (MP_TAC o
+                  SPECL[``A Delete1 (a:'a)``,``B Delete1 (a:'a)``]) o concl)
+        THEN RW_TAC arith_ss [Card1_Delete1,MEM_Delete1]
+        THEN POP_ASSUM (ASSUME_TAC o SPEC ``a:'a`` o MATCH_MP CONS_RSP)
+        THEN PROVE_TAC[MEM_CONS_Delete1,fset_SYM,fset_TRANS]
+      ]
+   );
+
+val list_EXTENSION = store_thm
+   ("list_EXTENSION",
+    ``!A B. A == B = (!a:'a. MEM a A = MEM a B)``,
+    PROVE_TAC[MEM_RSP,list_EXTENSION1]
+   );
+
+val Delete1_RSP = store_thm
+   ("Delete1_RSP",
+    ``!A B (a:'a). A == B ==>
+                     A Delete1 a == B Delete1 a``,
+    REWRITE_TAC [list_EXTENSION]
+    THEN REPEAT STRIP_TAC
+    THEN ASM_REWRITE_TAC [MEM_Delete1]
+   );
+
+val APPEND_RSP = store_thm
+   ("APPEND_RSP",
+    ``!A1 A2 B1 B2:'a list.
+           A1 == A2 /\ B1 == B2 ==>
+           APPEND A1 B1 == APPEND A2 B2``,
+    REWRITE_TAC[list_EXTENSION]
+    THEN REPEAT STRIP_TAC
+    THEN RW_TAC list_ss []
+   );
+
+val Inter1_def = Define
+   `($Inter1 ([]) B = [])  /\
+    ($Inter1 ((a:'a) :: A) B = if MEM a B then a :: ($Inter1 A B)
+                                          else $Inter1 A B)`;
+
+val _ = add_infix ("Inter1", 600, HOLgrammars.LEFT);
+
+val MEM_Inter1 = store_thm
+   ("MEM_Inter1",
+    ``!A B (x:'a).
+           MEM x (A Inter1 B) = MEM x A /\ MEM x B``,
+    Induct
+    THEN RW_TAC list_ss [Inter1_def]
+    THEN PROVE_TAC []
+   );
+
+val Inter1_RSP = store_thm
+   ("Inter1_RSP",
+    ``!A1 A2 B1 B2:'a list.
+           A1 == A2 /\ B1 == B2 ==>
+           A1 Inter1 B1 == A2 Inter1 B2``,
+    REWRITE_TAC[list_EXTENSION]
+    THEN REPEAT STRIP_TAC
+    THEN RW_TAC list_ss [Inter1_def,MEM_Inter1]
+   );
+
+(* --------------------------------------------------------------------- *)
+(* Definition of Fold1 function to fold a function over a finite set.    *)
+(* --------------------------------------------------------------------- *)
+
+val Fold1_def = Define
+   `(Fold1 f (g:'a->'b) (z:'b) ([]) = z)  /\
+    (Fold1 f g z (a :: A) =
+        if (!u v. f u v = f v u) /\
+           (!u v w. f u (f v w) = f (f u v) w)
+        then
+           if MEM a A then Fold1 f g z A
+                      else f (g a) (Fold1 f g z A)
+        else z)`;
+
+(* Respectfulness theorem for the Fold1 function. *)
+
+val Fold1_RSP = store_thm
+   ("Fold1_RSP",
+    ``!f (g:'a->'b) z A B. A == B ==>
+          (Fold1 f g z A = Fold1 f g z B)``,
+    GEN_TAC THEN GEN_TAC THEN GEN_TAC
+    THEN rule_induct fsequiv_strong_ind
+    THEN REPEAT STRIP_TAC
+    THEN REWRITE_TAC [Fold1_def]
+    THEN TRY COND_CASES_TAC
+    THEN PROVE_TAC[MEM,list_EXTENSION]
+   );
+
+(* --------------------------------------------------------------------- *)
+(* Definition of list2set function to convert a list to a set.           *)
+(* --------------------------------------------------------------------- *)
+
+val list2set_def = Define
+   `(list2set ([]) = {})  /\
+    (list2set ((a:'a) :: A) = a INSERT (list2set A))`;
+
+(* Respectfulness theorem for the list2set function. *)
+
+val list2set_RSP = store_thm
+   ("list2set_RSP",
+    ``!X Y:'a list. X == Y ==>
+          (list2set X = list2set Y)``,
+    rule_induct fsequiv_ind_thm
+    THEN REPEAT STRIP_TAC
+    THEN RW_TAC (std_ss ++ pred_setLib.PRED_SET_ss)
+                [list2set_def,INSERT_COMM,INSERT_INSERT]
+   );
+
+
+(* --------------------------------------------------------------------- *)
+(* Section 3, Lifting the finite set type and its constants.             *)
+(*                                                                       *)
+(* We first set up the parameters for the call to the tool, including    *)
+(* the equivalence relation on which the quotient is based, and the      *)
+(* list of constants to be lifted, with their new names and fixities.    *)
+(* --------------------------------------------------------------------- *)
+
+
+val fset_EQUIV = save_thm("fset_EQUIV",
+    refl_sym_trans_equiv fset_REFL fset_SYM fset_TRANS);
+
+val equivs = [fset_EQUIV];
+
+val fnlist =
+    [{def_name="Empty_def",
+      fname="Empty",
+      func= ``[] :'a list``,
+      fixity=Prefix},
+
+     {def_name="Insert_def",
+      fname="Insert",
+      func= ``CONS :'a -> 'a list -> 'a list``,
+      fixity=Infixr 490},
+
+     {def_name="In_def",
+      fname="In",
+      func= ``MEM :'a -> 'a list -> bool``,
+      fixity=Infix(NONASSOC,425)},
+
+     {def_name="Card_def",
+      fname="Card",
+      func= ``Card1 :'a list -> num``,
+      fixity=Prefix},
+
+     {def_name="Delete_def",
+      fname="Delete",
+      func= ``$Delete1 :'a list -> 'a -> 'a list``,
+      fixity=Infixl 500},
+
+     {def_name="Union_def",
+      fname="Union",
+      func= ``APPEND :'a list -> 'a list -> 'a list``,
+      fixity=Infixl 500},
+
+     {def_name="Inter_def",
+      fname="Inter",
+      func= ``$Inter1 :'a list -> 'a list -> 'a list``,
+      fixity=Infixl 600},
+
+     {def_name="Fold_def",
+      fname="Fold",
+      func= ``Fold1 :('b -> 'b -> 'b) -> ('a -> 'b) -> 'b -> 'a list -> 'b``,
+      fixity=Prefix},
+
+     {def_name="fset2set_def",
+      fname="fset2set",
+      func= ``list2set :'a list -> 'a -> bool``,
+      fixity=Prefix}
+    ];
+
+
+(* ==================================================== *)
+(*   LIFT TYPES, CONSTANTS, AND THEOREMS BY QUOTIENTS   *)
+(* ==================================================== *)
+
+val _ = quotient.chatting := true;   (* Causes display of quotient as built *)
+
+val  [finite_set_cases, Insert_LEFT_COMM, Insert_LEFT_IDEM,
+      In, NONE_In_Empty, In_Insert, finite_set_strong_cases,
+      Card, NOT_In_Card, Card_SUC, Card_Insert_GT_0,
+      In_Card_NOT_0, NOT_Empty_Insert,
+      Delete_def, In_Delete, Card_Delete,
+      Insert_Delete, In_Insert_Delete, finite_set_Delete_cases,
+      Union, In_Union, Inter, In_Inter,
+      Fold, fset2set, finite_set_EXTENSION, finite_set_INDUCT
+     ] =
+
+    define_quotient_types
+
+    {types = [{name = "finite_set", equiv = fset_EQUIV}],
+     defs = fnlist,
+     tyop_equivs = [],
+     tyop_quotients = [FUN_QUOTIENT],
+     tyop_simps = [FUN_REL_EQ, FUN_MAP_I],
+     respects = [NIL_RSP, CONS_RSP, MEM_RSP, Card1_RSP, Delete1_RSP,
+                 APPEND_RSP, Inter1_RSP, Fold1_RSP, list2set_RSP],
+     poly_preserves = [FORALL_PRS, EXISTS_PRS, COND_PRS],
+     poly_respects = [RES_FORALL_RSP, RES_EXISTS_RSP, COND_RSP],
+     old_thms = [list_CASES, CONS_LEFT_COMM, CONS_LEFT_IDEM,
+                 MEM, NONE_MEM_NIL, MEM_CONS, finite_set1_strong_cases,
+                 Card1_def, NOT_MEM_Card1, Card1_SUC, Card1_CONS_GT_0,
+                 MEM_Card1_NOT_0, NOT_NIL_EQUIV_CONS,
+                 Delete1_def, MEM_Delete1, Card1_Delete1,
+                 CONS_Delete1, MEM_CONS_Delete1, finite_set1_Delete1_cases,
+                 APPEND, MEM_APPEND, Inter1_def, MEM_Inter1,
+                 Fold1_def, list2set_def, list_EXTENSION, list_INDUCT]
+   };
+
+
+
+
+
+(* ---------------------------------------------------------------- *)
+(* Save the theorems lifted by the quotient operations.             *)
+(* ---------------------------------------------------------------- *)
+
+val _ = map save_thm
+    [("finite_set_cases",finite_set_cases),
+     ("Insert_LEFT_COMM",Insert_LEFT_COMM),
+     ("Insert_LEFT_IDEM",Insert_LEFT_IDEM),
+     ("In",In),
+     ("NONE_In_Empty",NONE_In_Empty),
+     ("In_Insert",In_Insert),
+     ("finite_set_strong_cases",finite_set_strong_cases),
+     ("Card",Card),
+     ("NOT_In_Card",NOT_In_Card),
+     ("Card_SUC",Card_SUC),
+     ("Card_Insert_GT_0",Card_Insert_GT_0),
+     ("In_Card_NOT_0",In_Card_NOT_0),
+     ("NOT_Empty_Insert",NOT_Empty_Insert),
+     ("Delete_def",Delete_def),
+     ("In_Delete",In_Delete),
+     ("Card_Delete",Card_Delete),
+     ("Insert_Delete",Insert_Delete),
+     ("In_Insert_Delete",In_Insert_Delete),
+     ("finite_set_Delete_cases",finite_set_Delete_cases),
+     ("Union",Union),
+     ("In_Union",In_Union),
+     ("Inter",Inter),
+     ("In_Inter",In_Inter),
+     ("Fold",Fold),
+     ("fset2set",fset2set),
+     ("finite_set_EXTENSION",finite_set_EXTENSION),
+     ("finite_set_INDUCT",finite_set_INDUCT)
+    ];
+
+(* Notice the important induction theorem for the quotient type:
+
+finite_set_INDUCT
+  |- !P. P Empty /\ (!f. P f ==> !a. P (a Insert f)) ==> !f. P f
+
+This is a higher-order theorem, which needs higher-order quotients
+to lift.  It is also interesting in that it is by this theorem
+an inductive type which was not defined inductively.
+*)
+
+
+(* ---------------------------------------------------------------- *)
+(*      End of saving important theorems from lifting.              *)
+(* ---------------------------------------------------------------- *)
+
+
+(* --------------------------------------------------------------------- *)
+(* Section 4, Exploitation of the new lifted type of finite sets.        *)
+(*                                                                       *)
+(* The rest of these proofs are achieved purely through reasoning at the *)
+(* higher, quotient level.  There is never again any need to deal with   *)
+(* concepts at the lower level, which may now be completely forgotten.   *)
+(* --------------------------------------------------------------------- *)
+
+(* Prove that the cardinality of a set may be expressed using Fold.      *)
+
+val Card_Fold = store_thm
+   ("Card_Fold",
+    ``Card = Fold $+ ((K 1):'a->num) 0``,
+    CONV_TAC FUN_EQ_CONV
+    THEN HO_MATCH_MP_TAC finite_set_INDUCT
+    THEN REPEAT STRIP_TAC
+    THEN RW_TAC arith_ss [Fold,Card]
+   );
+
+
+(* --------------------------------------------------------------------- *)
+(* Proof of stronger finite set induction principle.                     *)
+(* --------------------------------------------------------------------- *)
+
+val finite_set_strong_induction = store_thm
+   ("finite_set_strong_induction",
+    ``!P. P Empty /\
+            (!A. P A ==> !a:'a. ~(a In A) ==> P (a Insert A))
+            ==> !A. P A``,
+    GEN_TAC THEN STRIP_TAC
+    THEN HO_MATCH_MP_TAC finite_set_INDUCT
+    THEN PROVE_TAC [In_Insert]
+   );
+
+
+(*
+val fset2set_def =
+    |- (fset2set Empty = {}) /\
+       !a A. fset2set (a Insert A) = a INSERT fset2set A
+*)
+
+
+
+val IN_fset2set = store_thm
+   ("IN_fset2set",
+    ``!A (a:'a). a IN fset2set A = a In A``,
+    HO_MATCH_MP_TAC finite_set_INDUCT
+    THEN REPEAT STRIP_TAC
+    THEN RW_TAC (std_ss ++ pred_setLib.PRED_SET_ss) [fset2set,In]
+   );
+
+val fset2set_11 = store_thm
+   ("fset2set_11",
+    ``!A B:'a finite_set. (fset2set A = fset2set B) = (A = B)``,
+    REWRITE_TAC[finite_set_EXTENSION,EXTENSION,IN_fset2set]
+   );
+
+val fset2set_FINITE = store_thm
+   ("fset2set_FINITE",
+    ``!A:'a finite_set. FINITE (fset2set A)``,
+    HO_MATCH_MP_TAC finite_set_INDUCT
+    THEN REPEAT STRIP_TAC
+    THEN RW_TAC (std_ss ++ pred_setLib.PRED_SET_ss) [fset2set]
+   );
+
+val fset2set_ONTO_FINITE = store_thm
+   ("fset2set_ONTO_FINITE",
+    ``!s. FINITE s ==> ?A:'a finite_set. fset2set A = s``,
+    REWRITE_TAC[FINITE_DEF]
+    THEN GEN_TAC
+    THEN DISCH_THEN HO_MATCH_MP_TAC
+    THEN REPEAT STRIP_TAC
+    THEN PROVE_TAC[fset2set]
+   );
+
+(* So fset2set is a bijection between finite_set and finite pred_sets. *)
+
+val set2fset_def =
+    new_specification("set2fset_def",["set2fset"],
+         CONV_RULE (DEPTH_CONV RIGHT_IMP_EXISTS_CONV THENC SKOLEM_CONV)
+             fset2set_ONTO_FINITE);
+
+(*  |- !s. FINITE s ==> (fset2set (set2fset s) = s)      *)
+
+val set2fset_fset2set = store_thm
+   ("set2fset_fset2set",
+    ``!A:'a finite_set. set2fset (fset2set A) = A``,
+    GEN_TAC
+    THEN MP_TAC (MATCH_MP set2fset_def (SPEC_ALL fset2set_FINITE))
+    THEN REWRITE_TAC[fset2set_11]
+   );
+
+
+
+(* ===================================================================== *)
+(* End of the lifting of finite set types and definitions to the higher, *)
+(* more abstract level, where equivalent expressions are actually equal. *)
+(* ===================================================================== *)
+
+
+
+
+val _ = export_theory();
+
+val _ = print_theory_to_file "-" "finite_set.lst";
+
+val _ = html_theory "finite_set";
+
+fun print_theory_size () =
+   (print "The theory ";
+    print (current_theory ());
+    print " has ";
+    print (Int.toString (length (types (current_theory ()))));
+    print " types, ";
+    print (Int.toString (length (axioms "-")));
+    print " axioms, ";
+    print (Int.toString (length (definitions "-")));
+    print " definitions, and ";
+    print (Int.toString (length (theorems "-")));
+    print " theorems.";
+    print "\n" );
+
+val _ = print_theory_size();
